mm0-lean/x86/matching.lean
@@ -202,16 +202,6 @@ theorem block.read.stable {l v k k'}
   (h₁ : block.read l v k) (ss : places l ⊆ stability k k') :
   block.read l v k' := sorry
 
-inductive hoare_p (Q : kcfg → Prop) : kcfg → Prop
-| zero {{k}} : Q k → hoare_p k
-| step {{k}} : (∃ k', kcfg.step k k') →
-  (∀ k', k.step k' → hoare_p k') → hoare_p k
-| exit (k : kcfg) (ret) :
-  k.k.exit ret → (ret = 0 → Q k) → hoare_p k
-
-def hoare (P : kcfg → Prop) (Q : kcfg → kcfg → Prop) :=
-∀ {{k}}, P k → hoare_p (Q k) k
-
 def mHoareIO (P : sProp) (Q : list byte → list byte → mProp) :=
 hoare (λ k, P k.k)
   (λ k k', ∃ i' o', k.input = i' ++ k'.input ∧ k'.output = k.output ++ o' ∧
@@ -568,12 +558,7 @@ begin
   by_cases h_ret = 0,
   { cases H (h_a_1 h),
     { exact hoare_p.zero a },
-    { rcases a with ⟨_, ⟨_, _, _, _, h'⟩ | ⟨_, _, _, _, _, _, _, _, h'⟩⟩,
-      { cases config.step_no_exit h' h_a },
-      { rcases h_a with ⟨k₁, h₁, ⟨e⟩⟩,
-        cases config.isIO.determ h' h₁,
-        generalize_hyp : a_h_k₁.regs RAX = r at e a_h_a,
-        induction a_h_a; cases bitvec.reify_eq₂ e } },
+    { cases a with k' h, cases h.no_exit h_a },
     { exact hoare_p.exit _ _ a a_1 } },
   { exact hoare_p.exit _ _ h_a h.elim },
 end
@@ -860,10 +845,11 @@ stmt.hoare_iff.2 begin
     exact λ k, mem.read'_left ⟨_, rfl⟩ },
   rw [mProp.ex_apply, mHoare.ex_l], rintro (_|⟨n⟩),
   { refine ((stmt.hoare_iff.1 H₂ h₂).mono_l _).mono_r _,
-    rintro k₂ k₃ ⟨e₂, s₂, q₂, r₂⟩ e₁ k₁ ⟨s₁, q₁, r₁⟩,
-    rw [list.length_append, ← bitvec.add_nat_assoc],
-    refine ⟨e₂, s₁.trans s₂, _⟩,
-    exact ⟨⟨exit_kind.straight, _, q₁, q₂⟩, r₂⟩ },
+    { rintro k₂ k₃ ⟨e₂, s₂, q₂, r₂⟩ e₁ k₁ ⟨s₁, q₁, r₁⟩,
+      rw [list.length_append, ← bitvec.add_nat_assoc],
+      refine ⟨e₂, s₁.trans s₂, ⟨exit_kind.straight, _, _, q₂⟩, r₂⟩,
+      sorry },
+    { } },
   { exact ⟨⟨exit_kind.label n, q₁, _⟩, r₂⟩ },
 
   have:= (((stmt.hoare_iff.1 H₁ h₁).mono_l _).comp
